code/streaming/Hacl.Streaming.SHA2.fst
@@ -1,5 +1,10 @@
 module Hacl.Streaming.SHA2
 
+// NOTE: if you get errors trying to load this file in interactive mode because
+// a tactic fails in Hacl.Streaming.MD (even though Hacl.Streaming.MD works
+// totally fine in interactive mode!!), run:
+//     NODEPEND=1 make -j obj/Hacl.Streaming.MD.fst.checked
+
 open FStar.HyperStack.ST
 
 /// A streaming version of MD-based hashes
@@ -44,6 +49,19 @@ let state_sha2_256 = F.state_s hacl_sha2_256 () (state_t_256.s ()) (G.erased uni
 let state_sha2_384 = F.state_s hacl_sha2_384 () (state_t_384.s ()) (G.erased unit)
 let state_sha2_512 = F.state_s hacl_sha2_512 () (state_t_512.s ()) (G.erased unit)
 
+open Lib.Buffer
+open Lib.IntTypes
+
+// Slightly rewritten spec to remove any mention of multibuffer-isms
+inline_for_extraction noextract
+let hash_t (a: sha2_alg) =
+  dst:lbuffer uint8 (Hacl.Hash.Definitions.hash_len a) -> input_len:size_t -> input:lbuffer uint8 input_len ->
+    Stack unit
+    (requires fun h0 -> v input_len `less_than_max_input_length` a /\
+      live h0 input /\ live h0 dst /\ disjoint dst input)
+    (ensures  fun h0 _ h1 -> modifies (loc dst) h0 h1 /\
+      as_seq h1 dst == Spec.Agile.Hash.hash a (as_seq h0 input))
+
 inline_for_extraction noextract
 let alloca_224 = F.alloca hacl_sha2_224 () (state_t_224.s ()) (G.erased unit)
 let create_in_224 = F.create_in hacl_sha2_224 () (state_t_224.s ()) (G.erased unit)
@@ -52,6 +70,24 @@ let init_224 = F.init hacl_sha2_224 (G.hide ()) (state_t_224.s ()) (G.erased uni
 let update_224 = F.update hacl_sha2_224 (G.hide ()) (state_t_224.s ()) (G.erased unit)
 let finish_224 = F.mk_finish hacl_sha2_224 () (state_t_224.s ()) (G.erased unit)
 let free_224 = F.free hacl_sha2_224 (G.hide ()) (state_t_224.s ()) (G.erased unit)
+
+open Lib.NTuple
+open Lib.MultiBuffer
+open Hacl.Spec.SHA2.Vec
+open Hacl.SHA2.Scalar32
+open Hacl.Impl.SHA2.Generic
+module ST = FStar.HyperStack.ST
+
+val sha224: hash_t SHA2_224
+let sha224 dst input_len input =
+  let ib = ntup1 input in
+  let rb = ntup1 dst in
+  let h0 = ST.get() in
+  loc_multi1 rb;
+  hash #SHA2_224 #M32 sha224_init sha224_update_nblocks sha224_update_last sha224_finish rb input_len ib;
+  let h1 = ST.get() in
+  Hacl.Spec.SHA2.Equiv.hash_agile_lemma #SHA2_224 #M32 (v input_len) (as_seq_multi h0 ib);
+  assert ((as_seq_multi h1 rb).(|0|) == as_seq h1 dst)
 
 inline_for_extraction noextract
 let alloca_256 = F.alloca hacl_sha2_256 () (state_t_256.s ()) (G.erased unit)
@@ -62,6 +98,17 @@ let update_256 = F.update hacl_sha2_256 (G.hide ()) (state_t_256.s ()) (G.erased
 let finish_256 = F.mk_finish hacl_sha2_256 () (state_t_256.s ()) (G.erased unit)
 let free_256 = F.free hacl_sha2_256 (G.hide ()) (state_t_256.s ()) (G.erased unit)
 
+val sha256: hash_t SHA2_256
+let sha256 dst input_len input =
+  let ib = ntup1 input in
+  let rb = ntup1 dst in
+  let h0 = ST.get() in
+  loc_multi1 rb;
+  hash #SHA2_256 #M32 sha256_init sha256_update_nblocks sha256_update_last sha256_finish rb input_len ib;
+  let h1 = ST.get() in
+  Hacl.Spec.SHA2.Equiv.hash_agile_lemma #SHA2_256 #M32 (v input_len) (as_seq_multi h0 ib);
+  assert ((as_seq_multi h1 rb).(|0|) == as_seq h1 dst)
+
 inline_for_extraction noextract
 let alloca_384 = F.alloca hacl_sha2_384 () (state_t_384.s ()) (G.erased unit)
 let create_in_384 = F.create_in hacl_sha2_384 () (state_t_384.s ()) (G.erased unit)
@@ -71,6 +118,17 @@ let update_384 = F.update hacl_sha2_384 (G.hide ()) (state_t_384.s ()) (G.erased
 let finish_384 = F.mk_finish hacl_sha2_384 () (state_t_384.s ()) (G.erased unit)
 let free_384 = F.free hacl_sha2_384 (G.hide ()) (state_t_384.s ()) (G.erased unit)
 
+val sha384: hash_t SHA2_384
+let sha384 dst input_len input =
+  let ib = ntup1 input in
+  let rb = ntup1 dst in
+  let h0 = ST.get() in
+  loc_multi1 rb;
+  hash #SHA2_384 #M32 sha384_init sha384_update_nblocks sha384_update_last sha384_finish rb input_len ib;
+  let h1 = ST.get() in
+  Hacl.Spec.SHA2.Equiv.hash_agile_lemma #SHA2_384 #M32 (v input_len) (as_seq_multi h0 ib);
+  assert ((as_seq_multi h1 rb).(|0|) == as_seq h1 dst)
+
 inline_for_extraction noextract
 let alloca_512 = F.alloca hacl_sha2_512 () (state_t_512.s ()) (G.erased unit)
 let create_in_512 = F.create_in hacl_sha2_512 () (state_t_512.s ()) (G.erased unit)
@@ -79,3 +137,14 @@ let init_512 = F.init hacl_sha2_512 (G.hide ()) (state_t_512.s ()) (G.erased uni
 let update_512 = F.update hacl_sha2_512 (G.hide ()) (state_t_512.s ()) (G.erased unit)
 let finish_512 = F.mk_finish hacl_sha2_512 () (state_t_512.s ()) (G.erased unit)
 let free_512 = F.free hacl_sha2_512 (G.hide ()) (state_t_512.s ()) (G.erased unit)
+
+val sha512: hash_t SHA2_512
+let sha512 dst input_len input =
+  let ib = ntup1 input in
+  let rb = ntup1 dst in
+  let h0 = ST.get() in
+  loc_multi1 rb;
+  hash #SHA2_512 #M32 sha512_init sha512_update_nblocks sha512_update_last sha512_finish rb input_len ib;
+  let h1 = ST.get() in
+  Hacl.Spec.SHA2.Equiv.hash_agile_lemma #SHA2_512 #M32 (v input_len) (as_seq_multi h0 ib);
+  assert ((as_seq_multi h1 rb).(|0|) == as_seq h1 dst)
